zab model

zab.dfy
@@ -1,170 +1,167 @@
 datatype St  = L | F | R | S
-datatype Msg = BROADCAST(m: int) |
-  ACCEPT(b: int, k: int, m: int) |
-  ACCEPT_ACK(b: int, k: int, m: int, s: int) |
-  COMMIT(b: int, k: int, m: int) |
-  DELIVER(k: int, m: int, s: int) |
-  NEW_LEADER(b: int) |
-  NEW_LEADER_ACK(b: int, c: int, log: map<int, int>, s: int) |
-  NEW_STATE(b: int, log: map<int, int>) |
-  NEW_STATE_ACK(b: int, s: int)
 
-	method pick_with_max_cbal_and_len(acks: set<Msg>) returns (m: Msg)
+datatype Msg = BROADCAST(m: int) |
+               ACCEPT(b: int, k: int, m: int) |
+               ACCEPT_ACK(b: int, k: int, m: int, s: int) |
+               COMMIT(b: int, k: int, m: int) |
+               NEW_LEADER(b: int) |
+               NEW_LEADER_ACK(b: int, c: int, log: map<int, int>, s: int) |
+               NEW_STATE(b: int, log: map<int, int>) |
+               NEW_STATE_ACK(b: int, s: int)
+
+method pick_with_max_cbal_and_len(acks: set<Msg>) returns (m: Msg)
     requires acks != {}
     requires forall m :: m in acks ==> m.NEW_LEADER_ACK?
-			ensures m in acks && m.NEW_LEADER_ACK?
-			ensures forall m' :: m' in acks ==> m'.c < m.c || (m'.c == m.c && |m'.log| <= |m.log|)
-	{
+    ensures m in acks
+    ensures forall m' :: m' in acks ==> m'.c < m.c || (m'.c == m.c && |m'.log| <= |m.log|)
+{
     m :| m in acks;
     var q', q := {m}, acks - {m};
     while (q != {})
-      decreases q
-      invariant q + q' == acks
-      invariant m in acks && m.NEW_LEADER_ACK?
-      invariant forall m' :: m' in q' ==>  m'.c < m.c || (m'.c == m.c && |m'.log| <= |m.log|)
+        decreases q
+        invariant q + q' == acks
+        invariant m in acks
+        invariant forall m' :: m' in q' ==>  m'.c < m.c || (m'.c == m.c && |m'.log| <= |m.log|)
     {
-      var y :| y in q;
-      q, q' := q - {y}, q' + {y};
-      if (m.c < y.c || (m.c == y.c && |y.log| > |m.log|)) {
-        m := y;
-      }
+        var y :| y in q;
+        q, q' := q - {y}, q' + {y};
+        if (m.c < y.c || (m.c == y.c && |y.log| > |m.log|)) {
+            m := y;
+        }
     }
-	}
-  
-	method new_bal(b: int, p: int, N: int) returns (b': int)
+}
+
+method new_bal(b: int, p: int, N: int) returns (b': int)
     requires b >= -1 && N > 0
     ensures b' > b && b' % N == p
     decreases *
-	{
+{
     b' := b + 1;
     while (b' % N != p)
-      decreases *
-      invariant b' > b
+        decreases *
+        invariant b' > b
     {
-      b' := b' + 1;
+        b' := b' + 1;
     }
-	}
+}
 
-	method zab(ps: set<int>, N: int)
+predicate is_prefix(s: seq<Msg>, s': seq<Msg>)
+{
+    |s| <= |s'| && forall i :: 0 <= i < |s| ==> s[i] == s'[i]
+}
+
+method zab(ps: set<int>, N: int)
     requires N > 0 && |ps| == N
     requires forall p :: p in ps ==> 0 <= p < N
     decreases *
-	{
-    var st:             map<int, St>            := map p | p in ps ::     F;
-    var log:            map<int, map<int, int>> := map p | p in ps :: map[];
-    var bal:            map<int, int>           := map p | p in ps ::    -1;
-    var cbal:           map<int, int>           := map p | p in ps ::    -1;
-    var next_send:      map<int, int>           := map p | p in ps ::    -1;
-    var next_recv:      map<int, int>           := map p | p in ps ::    -1;
-    var last_delivered: map<int, int>           := map p | p in ps ::    -1;
+{
+    var st: map<int, St> := map p | p in ps :: F;
+    var log: map<int, map<int, int>> := map p | p in ps :: map[];
+    var bal: map<int, int> := map p | p in ps :: -1;
+    var cbal: map<int, int> := map p | p in ps :: -1;
+    var next: map<int, int> := map p | p in ps :: 0;
 
-    var accept_acks:     map<int, set<Msg>> := map p | p in ps :: {};
+    var last_delivered: map<int, int> := map p | p in ps :: -1;
+    var dlog: map<int, seq<Msg>> := map p | p in ps :: [];
+
+    var accept_acks: map<int, map<int, set<Msg>>> := map p | p in ps :: map[];
     var new_leader_acks: map<int, set<Msg>> := map p | p in ps :: {};
-    var new_state_acks:  map<int, set<Msg>> := map p | p in ps :: {};
+    var new_state_acks: map<int, set<Msg>> := map p | p in ps :: {};
 
     var ios: set<Msg> := {};
 
-    ghost var accepts:     map<int, set<Msg>>      := map p | p in ps ::    {};
-    ghost var initial_msg: map<int, map<int, int>> := map p | p in ps :: map[];
+    while (true)
+        decreases *
 
-    ghost var ios': set<Msg>;
-    ghost var bal': map<int, int>;
+        invariant st.Keys == log.Keys == bal.Keys == cbal.Keys == next.Keys ==
+                  last_delivered.Keys == dlog.Keys == accept_acks.Keys ==
+                  new_leader_acks.Keys == new_state_acks.Keys == ps
 
-    while true
-      decreases *
+        invariant forall p :: p in ps ==> bal[p] >= -1
+        invariant forall p, m :: p in ps && m in new_state_acks[p]  ==> m.NEW_STATE_ACK?
+        invariant forall p, m :: p in ps && m in new_leader_acks[p] ==> m.NEW_LEADER_ACK?
+        invariant forall p, m, k :: p in ps && k in accept_acks[p] && m in accept_acks[p][k] ==> m.ACCEPT_ACK?
 
-      invariant st.Keys == log.Keys == bal.Keys == cbal.Keys == next_send.Keys ==
-      next_recv.Keys == last_delivered.Keys == accept_acks.Keys ==
-      new_leader_acks.Keys == new_state_acks.Keys == accepts.Keys ==
-      initial_msg.Keys == ps
-
-      invariant forall p, m :: p in ps && m in accept_acks[p] ==> m.ACCEPT_ACK?
-      invariant forall p, m :: p in ps && m in new_leader_acks[p] ==> m.NEW_LEADER_ACK?
-      invariant forall p, m :: p in ps && m in new_state_acks[p] ==> m.NEW_STATE_ACK?
-
-      invariant forall p :: p in ps ==> bal[p] >= -1          
     {
-      bal' := bal; ios' := ios;
+        var p :| p in ps;
+        var recover :| recover in {false, true};
 
-      var p       :| p in ps;
-      var recover :| recover in {false, true};
-
-      if recover {
-        var b := new_bal(bal[p], p, N);
-        ios := ios + { NEW_LEADER(bal[p]) };
-      } else {
-        var bcast :| bcast in {false, true};
-
-        if ((st[p] == L && bcast) || ios == {}) {
-          next_send := next_send[p := next_send[p] + 1];
-          var m: int := *;
-          var tmp := log[p][next_send[p] := m];
-          log := log[p := tmp];
-          accept_acks := accept_acks[p := {}];
-          ios := ios + { ACCEPT(bal[p], next_send[p], m) };
+        if (recover || ios == {}) {
+            var b := new_bal(bal[p], p, N);
+            new_leader_acks := new_leader_acks[p := {}];
+            ios := ios + {NEW_LEADER(b)};
         } else {
-          var msg :| msg in ios;
+            var bcast :| bcast in {false, true};
 
-          if (msg.ACCEPT? && st[p] in {L, F} && msg.b == bal[p] && msg.k == next_recv[p]) {
-            var tmp := log[p][msg.k := msg.m];
-            log := log[p := tmp];
-            next_recv := next_recv[p := next_recv[p] + 1];
-            ios  := ios + { ACCEPT_ACK(msg.b, msg.k, msg.m, p) };
-          }
+            if (st[p] == L && bcast) {
+                var m: int := *;
+                log := log[p := log[p][next[p] := m]];
+                next := next[p := next[p] + 1];
+                accept_acks := accept_acks[p := accept_acks[p][next[p] := {}]];
+                ios := ios + {ACCEPT(bal[p], next[p] - 1, m)};
+            } else {
+                var msg :| msg in ios;
 
-          if (msg.ACCEPT_ACK? && st[p] == L && msg.b == bal[p]) {
-            var tmp := accept_acks[p] + { msg };
-            accept_acks := accept_acks[p := tmp];
-            var A' := set m | m in accept_acks[p] :: m.s;
-            if (2 * |A'| > N) {
-              ios := ios + { COMMIT(msg.b, msg.k, msg.m) };
+                if (msg.ACCEPT? && st[p] in {L, F} && msg.b == bal[p]) {
+                    assume msg.k == |log[p]|;
+                    log := log[p := log[p][msg.k := msg.m]];
+                    ios := ios + {ACCEPT_ACK(msg.b, msg.k, msg.m, p)};
+                }
+
+                if (msg.ACCEPT_ACK? && st[p] == L && msg.b == bal[p]) {
+                    assume msg.k in accept_acks[p];
+                    accept_acks := accept_acks[p := accept_acks[p][msg.k := accept_acks[p][msg.k] + {msg}]];
+                    var A' := set m | m in accept_acks[p][msg.k] :: m.s;
+                    if (2 * |A'| > N) {
+                        ios := ios + {COMMIT(msg.b, msg.k, msg.m)};
+                    }
+                }
+
+                if (msg.COMMIT? && st[p] in {L, F} && bal[p] >= msg.b && last_delivered[p] < msg.k) {
+                    assume msg.k <= |log[p]|;
+                    last_delivered := last_delivered[p := msg.k];
+                    log := log[p := log[p][msg.k := msg.m]];
+                    dlog := dlog[p := dlog[p] + [msg]];
+                }
+
+                if (msg.NEW_LEADER? && msg.b > bal[p]) {
+                    st := st[p := R];
+                    bal := bal[p := msg.b];
+                    ios := ios + {NEW_LEADER_ACK(bal[p], cbal[p], log[p], p)};
+                }
+
+                if (msg.NEW_LEADER_ACK? && st[p] == R && msg.b == bal[p]) {
+                    new_leader_acks := new_leader_acks[p := new_leader_acks[p] + {msg}];
+                    var A' := set m | m in new_leader_acks[p] :: m.s;
+                    if (2 * |A'| > N) {
+                        var m := pick_with_max_cbal_and_len(new_leader_acks[p]);
+                        cbal := cbal[p := bal[p]];
+                        log := log[p := m.log];
+                        next := next[p := |log[p]|];
+                        st := st[p := S];
+                        new_state_acks := new_state_acks[p := {}];
+                        ios := ios + {NEW_STATE(bal[p], log[p])};
+                    }
+                }
+
+                if (msg.NEW_STATE? && msg.b >= bal[p]) {
+                    bal := bal[p := msg.b];
+                    cbal := cbal[p := msg.b];
+                    log := log[p := msg.log];
+                    st := st[p := F];
+                    ios := ios + {NEW_STATE_ACK(bal[p], p)};
+                }
+
+                if (msg.NEW_STATE_ACK? && st[p] == S && bal[p] == msg.b) {
+                    new_state_acks := new_state_acks[p := new_state_acks[p] + {msg}];
+                    var A' := (set m | m in new_state_acks[p] :: m.s) + {p};
+                    if (2 * |A'| > N) {
+                        st := st[p := L];
+                        ios := ios + (set k | k in log[p] :: COMMIT(bal[p], k, log[p][k]));
+                    }
+                }
             }
-          }
-
-          if (msg.COMMIT? && st[p] in {L, F} && bal[p] >= msg.b && last_delivered[p] < msg.k) {
-            last_delivered := last_delivered[p := msg.k];
-            var tmp := log[p][msg.k := msg.m];
-            log := log[p := tmp];
-            ios := ios + { DELIVER(msg.k, msg.m, p) };
-          }
-
-          if (msg.NEW_LEADER? && msg.b > bal[p]) {
-            st := st[p := R];
-            bal := bal[p := msg.b];
-            ios := ios + { NEW_LEADER_ACK(bal[p], cbal[p], log[p], p) };
-          }
-
-          if (msg.NEW_LEADER_ACK? && st[p] == R && msg.b == bal[p]) {
-            var tmp := new_leader_acks[p] + { msg };
-            new_leader_acks := new_leader_acks[p := tmp];
-            var A' := set m | m in new_leader_acks[p] :: m.s;
-            if (2 * |A'| > N) {
-              var m := pick_with_max_cbal_and_len(new_leader_acks[p]);
-              cbal := cbal[p := bal[p]];
-              log := log[p := m.log];
-              next_send := next_send[p := |m.log| + 1];
-              st := st[p := S];
-              ios := ios + { NEW_STATE(bal[p], log[p]) };
-            }
-          }
-
-          if (msg.NEW_STATE? && msg.b >= bal[p]) {
-            bal := bal[p := msg.b];
-            cbal := cbal[p := msg.b];
-            log := log[p := msg.log];
-            st := st[p := F];
-            ios := ios + { NEW_STATE_ACK(bal[p], p) };
-          }
-
-          if (msg.NEW_STATE_ACK? && st[p] == S && bal[p] == msg.b) {
-            var tmp := new_state_acks[p] + { msg };
-            var A' := (set m | m in new_state_acks[p] :: m.s) + { p };
-            if (2 * |A'| > N) {
-              st := st[p := L];
-              ios := ios + (set k | k in log[p] :: COMMIT(bal[p], k, log[p][k]));
-            }
-          }
         }
-      }
     }
-	}
+}
+
